NCML.lean
@@ -4,6 +4,7 @@ public import NCML.CK.Canonical
 public import NCML.CK.Countermodel.BBox
 public import NCML.CK.Countermodel.ReturningMRel
 public import NCML.CK.Countermodel.SerialMRel
+public import NCML.CK.Countermodel.T
 public import NCML.CK.Countermodel.TDia
 public import NCML.CK.Frame.BBox
 public import NCML.CK.Frame.BDia
@@ -15,16 +16,19 @@ public import NCML.CK.Frame.ForwardConfluent
 public import NCML.CK.Frame.FourBox
 public import NCML.CK.Frame.FourDia
 public import NCML.CK.Frame.PBox
+public import NCML.CK.Frame.ReflexiveMRel
 public import NCML.CK.Frame.ReturningMRel
 public import NCML.CK.Frame.SerialMRel
 public import NCML.CK.Frame.StrictlyAscendingMRel
 public import NCML.CK.Frame.SymmetricMRel
+public import NCML.CK.Frame.T
 public import NCML.CK.Frame.TBox
 public import NCML.CK.Frame.TDia
 public import NCML.CK.Frame.TransitiveMRel
 public import NCML.CK.Logic.CK
 public import NCML.CK.Logic.CKB
 public import NCML.CK.Logic.CKD
+public import NCML.CK.Logic.CKT
 public import NCML.CK.Logic.CKTBox
 public import NCML.CK.Logic.CKTDia
 public import NCML.CK.Semantics
