NCML/CK/Frame/ReflexiveMRel.lean
@@ -1,0 +1,34 @@
+module
+
+public import NCML.CK.Frame.ReturningMRel
+public import NCML.CK.Frame.StrictlyAscendingMRel
+public import NCML.CK.Frame.T
+
+@[expose] public section
+
+namespace CK
+
+variable {κ : Type*}
+
+namespace Frame
+
+variable {F : Frame κ}
+
+class ReflexiveMRel (F : Frame κ) : Prop where
+  refl_mRel : ∀ x : F.World, x ⊏ x
+
+export ReflexiveMRel (refl_mRel)
+
+instance [F.ReflexiveMRel] : F.ReturningMRel where
+  returning_mRel x := ⟨x, refl x, refl_mRel x⟩
+
+instance [F.ReflexiveMRel] : F.StrictlyAscendingMRel where
+  strictly_ascending_mRel x := ⟨x, refl_mRel x, refl x⟩
+
+instance [F.ReflexiveMRel] : F.T where
+
+end Frame
+
+end CK
+
+end
