NCML/CK/Frame/T.lean
@@ -1,0 +1,44 @@
+module
+
+public import NCML.CK.Frame.TBox
+public import NCML.CK.Frame.TDia
+
+@[expose] public section
+
+namespace CK
+
+variable {κ : Type*}
+variable {A : BDFormula}
+
+namespace Frame
+
+variable {F : Frame κ}
+
+class T (F : Frame κ) : Prop extends TBox F, TDia F
+
+lemma frameValidate_T_of_frame_T [F.T] : F ⊧ ((□A 🡒 A) ⋏ (A 🡒 ◇A)) := by
+  intro V V_per V_fal x;
+  exact ⟨
+    frameValidate_TBox_of_frame_TBox V V_per V_fal x,
+    frameValidate_TDia_of_frame_TDia V V_per V_fal x
+  ⟩;
+
+lemma frame_T_of_frameValidate_T (h : F ⊧ ((□(#0) 🡒 #0) ⋏ (#0 🡒 ◇(#0)))) : F.T where
+  toTBox := frame_TBox_of_frameValidate_TBox (fun V V_per V_fal x => (h V V_per V_fal x).1)
+  toTDia := frame_TDia_of_frameValidate_TDia (fun V V_per V_fal x => (h V V_per V_fal x).2)
+
+theorem frame_T_TFAE : List.TFAE [
+  F.T,
+  ∀ A : BDFormula, F ⊧ ((□A 🡒 A) ⋏ (A 🡒 ◇A)),
+  F ⊧ ((□(#0) 🡒 #0) ⋏ (#0 🡒 ◇(#0))),
+] := by
+  tfae_have 1 → 2 := by intro h A; exact frameValidate_T_of_frame_T;
+  tfae_have 2 → 3 := fun h => h _
+  tfae_have 3 → 1 := frame_T_of_frameValidate_T
+  tfae_finish
+
+end Frame
+
+end CK
+
+end
