NCML/CK/Logic/CKT.lean
@@ -1,0 +1,61 @@
+module
+
+public import NCML.CK.Frame.ReflexiveMRel
+public import NCML.CK.Logic.CKTBox
+public import NCML.CK.Logic.CKTDia
+
+@[expose] public section
+
+instance : LogicCKT.TBox := ⟨LogicCKT.provable_TBox⟩
+instance : LogicCKT.TDia := ⟨LogicCKT.provable_TDia⟩
+
+open ProvableBDHilbert
+open scoped BDFormulaSet BDFormulaList
+
+namespace CK
+
+variable {κ : Type*} {M : Model κ}
+variable {A : BDFormula}
+
+namespace Model
+
+open CK.Frame
+
+lemma valid_of_mem_LogicCKT [M.T] (hA : A ∈ LogicCKT) : M ⊧ A :=
+  valid_of_mem_logic (by
+    rintro B (⟨C, rfl⟩ | ⟨C, rfl⟩);
+    · exact valid_of_toFrame_valid frameValidate_TBox_of_frame_TBox;
+    · exact valid_of_toFrame_valid frameValidate_TDia_of_frame_TDia;
+  ) hA
+
+end Model
+
+variable {L : BDLogic} [L.CK]
+
+instance reflexiveMRel_canonicalModel [L.TBox] [L.TDia] : (canonicalModel L).ReflexiveMRel where
+  refl_mRel P := ⟨
+    fun _ hA => P.theory.mdp (P.theory.subset L.tBox) hA,
+    fun _ hB => CanonicalPair.forbidden_not_mem_theory hB
+  ⟩
+
+end CK
+
+theorem LogicCKT_TFAE {A : BDFormula} : List.TFAE [
+  A ∈ LogicCKT,
+  ∀ {κ : Type 0}, ∀ F : CK.Frame κ, [F.T] → F ⊧ A,
+  ∀ {κ : Type 0}, ∀ F : CK.Frame κ, [F.ReflexiveMRel] → F ⊧ A,
+] := by
+  tfae_have 1 → 2 := fun h _ F _ V V_per V_fal => CK.Model.valid_of_mem_LogicCKT h
+  tfae_have 2 → 3 := fun h _ F _ => h F
+  tfae_have 3 → 1 := by
+    contrapose!;
+    intro h;
+    obtain ⟨P, h₁⟩ := CK.exists_not_forces_of_not_mem h;
+    refine ⟨_, (CK.canonicalModel LogicCKT).toFrame, ?_⟩;
+    and_intros;
+    . infer_instance;
+    . by_contra! hF;
+      exact h₁ $ CK.Model.valid_of_toFrame_valid hF P;
+  tfae_finish
+
+end
